user 3, session 5567, part 8

diffs-annotated-fixed/3/user-3-session-5567.v
@@ -173,6 +173,8 @@ step.
 {
 (destruct r; step).
 -
+(destruct r; step).
+-
 (descend; intuition eauto).
 {
 (destruct (lt_dec a (diskSize a'))).
@@ -185,11 +187,395 @@ step.
 (destruct r; intuition eauto; simplify).
 -
 (destruct r; step).
-Add Search Blacklist "Raw" "Proofs".
-Set Search Output Name Only.
-Redirect "/var/folders/5x/1mdbpbjd7012l971fq0zkj2w0000gn/T/coqpDheCv"
-SearchPattern _.
-Remove Search Blacklist "Raw" "Proofs".
-Unset Search Output Name Only.
+Qed.
+Hint Resolve write_int_ok: core.
+Theorem size_int_ok :
+  proc_spec
+    (fun '(d_0, d_1) state =>
+     {|
+     pre := disk0 state ?|= eq d_0 /\
+            disk1 state ?|= eq d_1 /\ diskSize d_0 = diskSize d_1;
+     post := fun r state' =>
+             r = diskSize d_0 /\
+             r = diskSize d_1 /\
+             disk0 state' ?|= eq d_0 /\ disk1 state' ?|= eq d_1;
+     recovered := fun _ state' =>
+                  disk0 state' ?|= eq d_0 /\ disk1 state' ?|= eq d_1 |}) size
+    td.recover td.abstr.
+Proof.
+(unfold size).
+step.
+(destruct r; step).
+(destruct r; step).
+Qed.
+Hint Resolve size_int_ok: core.
+Definition equal_after a (d_0 d_1 : disk) :=
+  diskSize d_0 = diskSize d_1 /\
+  (forall a', a <= a' -> diskGet d_0 a' = diskGet d_1 a').
+Theorem le_eq_or_S_le : forall n m, n <= m -> n = m \/ S n <= m /\ n <> m.
+Proof.
+(intros).
+lia.
+Qed.
+Theorem equal_after_diskUpd :
+  forall a d_0 d_1 b,
+  equal_after (S a) d_0 d_1 ->
+  equal_after a (diskUpd d_0 a b) (diskUpd d_1 a b).
+Proof.
+(unfold equal_after; intuition).
+-
+(autorewrite with upd; eauto).
+-
+(apply le_eq_or_S_le in H1; intuition subst).
+{
+(destruct (lt_dec a' (diskSize d_0)); autorewrite with upd).
++
+(assert (a' < diskSize d_1) by congruence; autorewrite with upd; auto).
++
+(assert (~ a' < diskSize d_1) by congruence; autorewrite with upd; auto).
+}
+(autorewrite with upd; eauto).
+Qed.
+Hint Resolve equal_after_diskUpd: core.
+Theorem init_at_ok :
+  forall a,
+  proc_spec
+    (fun '(d_0, d_1) state =>
+     {|
+     pre := disk0 state ?|= eq d_0 /\
+            disk1 state ?|= eq d_1 /\ equal_after a d_0 d_1;
+     post := fun _ state' =>
+             exists d_0' d_1' : disk,
+               disk0 state' ?|= eq d_0' /\
+               disk1 state' ?|= eq d_1' /\ equal_after 0 d_0' d_1';
+     recovered := fun _ state' => True |}) (init_at a) td.recover td.abstr.
+Proof.
+(induction a; simpl; intros).
+-
+step.
+-
+step.
+step.
+(destruct r; finish).
++
+step.
+(destruct r; simplify; finish).
++
+step.
+(destruct r; finish).
+Qed.
+Hint Resolve init_at_ok: core.
+Theorem sizeInit_ok :
+  proc_spec
+    (fun '(d_0, d_1) state =>
+     {|
+     pre := disk0 state ?|= eq d_0 /\ disk1 state ?|= eq d_1;
+     post := fun r state' =>
+             exists d_0' d_1',
+               disk0 state' ?|= eq d_0' /\
+               disk1 state' ?|= eq d_1' /\
+               match r with
+               | Some sz => diskSize d_0' = sz /\ diskSize d_1' = sz
+               | None => True
+               end;
+     recovered := fun _ state' => True |}) sizeInit td.recover td.abstr.
+Proof.
+(unfold sizeInit).
+step.
+(destruct r).
+-
+step.
+(destruct r).
++
+(destruct (diskSize d_0 == v)).
+*
+step.
+*
+step.
++
+step.
+-
+step.
+(destruct r).
++
+step.
++
+step.
+Qed.
+Hint Resolve sizeInit_ok: core.
+Theorem equal_after_0_to_eq :
+  forall d_0 d_1, equal_after 0 d_0 d_1 -> d_0 = d_1.
+Proof.
+(unfold equal_after; intuition).
+(eapply disk_ext_eq; intros).
+(eapply H0; lia).
+Qed.
+Theorem equal_after_size :
+  forall d_0 d_1,
+  diskSize d_0 = diskSize d_1 -> equal_after (diskSize d_0) d_0 d_1.
+Proof.
+(unfold equal_after; intuition).
+(assert (~ a' < diskSize d_0) by lia).
+(assert (~ a' < diskSize d_1) by congruence).
+(autorewrite with upd; eauto).
+Qed.
+Hint Resolve equal_after_size: core.
+Hint Resolve equal_after_0_to_eq: core.
+Theorem init'_ok :
+  proc_spec
+    (fun '(d_0, d_1) state =>
+     {|
+     pre := disk0 state ?|= eq d_0 /\ disk1 state ?|= eq d_1;
+     post := fun r state' =>
+             match r with
+             | Initialized =>
+                 exists d_0' d_1',
+                   disk0 state' ?|= eq d_0' /\
+                   disk1 state' ?|= eq d_1' /\ d_0' = d_1'
+             | InitFailed => True
+             end;
+     recovered := fun _ state' => True |}) init' td.recover td.abstr.
+Proof.
+(unfold init).
+step.
+(descend; intuition eauto).
+(destruct r; step).
+step.
+Qed.
+Hint Resolve init'_ok: core.
+Inductive RecStatus :=
+  | Continue : _
+  | RepairDoneOrFailed : _.
+Definition fixup (a : addr) : proc RecStatus :=
+  mv0 <- td.read d0 a;
+  match mv0 with
+  | Working v =>
+      mv2 <- td.read d1 a;
+      match mv2 with
+      | Working v' =>
+          if v == v'
+          then Ret Continue
+          else mu <- td.write d1 a v; Ret RepairDoneOrFailed
+      | Failed => Ret RepairDoneOrFailed
+      end
+  | Failed => Ret RepairDoneOrFailed
+  end.
+Definition fixup_stub (a : addr) : proc RecStatus := Ret Continue.
+Fixpoint recover_at (a : addr) : proc unit :=
+  match a with
+  | 0 => Ret tt
+  | S n =>
+      s <- fixup n;
+      match s with
+      | Continue => recover_at n
+      | RepairDoneOrFailed => Ret tt
+      end
+  end.
+Definition Recover : proc unit := sz <- size; _ <- recover_at sz; Ret tt.
+Theorem if_lt_dec :
+  forall A n m (a a' : A), n < m -> (if lt_dec n m then a else a') = a.
+Proof.
+(intros).
+(destruct (lt_dec n m); auto).
+Qed.
+Theorem disks_eq_inbounds :
+  forall (d : disk) a v v',
+  a < diskSize d -> diskGet d a =?= v -> diskGet d a =?= v' -> v = v'.
+Proof.
+(intros).
+(case_eq (diskGet d a); intros).
+-
+(rewrite H2 in *).
+(simpl in *).
+congruence.
+-
+exfalso.
+(eapply disk_inbounds_not_none; eauto).
+Qed.
+Inductive DiskStatus :=
+  | FullySynced : _
+  | OutOfSync : forall (a : addr) (b : block), _.
+Theorem diskUpd_maybe_same :
+  forall (d : disk) a b, diskGet d a =?= b -> diskUpd d a b = d.
+Proof.
+(intros).
+(destruct (diskGet d a) eqn:?; simpl in *; subst; autorewrite with upd; auto).
+Qed.
+Hint Rewrite diskUpd_maybe_same using (solve [ auto ]) : upd.
+Hint Resolve PeanoNat.Nat.lt_neq: core.
+Hint Resolve disks_eq_inbounds: core.
+Theorem fixup_equal_ok :
+  forall a,
+  proc_spec
+    (fun d state =>
+     {|
+     pre := a < diskSize d /\ disk0 state ?|= eq d /\ disk1 state ?|= eq d;
+     post := fun r state' => disk0 state' ?|= eq d /\ disk1 state' ?|= eq d;
+     recovered := fun _ state' =>
+                  disk0 state' ?|= eq d /\ disk1 state' ?|= eq d |})
+    (fixup a) td.recover td.abstr.
+Proof.
+(unfold fixup).
+step.
+(destruct r; step).
+(destruct r; try step).
+(destruct (v == v0); subst; try step).
+Unshelve.
+{
+auto.
+}
+exact (fun _ => True).
+Qed.
+Theorem fixup_correct_addr_ok :
+  forall a,
+  proc_spec
+    (fun '(d, b) state =>
+     {|
+     pre := a < diskSize d /\
+            disk0 state ?|= eq (diskUpd d a b) /\ disk1 state ?|= eq d;
+     post := fun r state' =>
+             match r with
+             | Continue =>
+                 disk0 state' ?|= eq (diskUpd d a b) /\
+                 disk1 state' ?|= eq (diskUpd d a b)
+             | RepairDoneOrFailed =>
+                 disk0 state' ?|= eq (diskUpd d a b) /\
+                 disk1 state' ?|= eq (diskUpd d a b) \/
+                 disk0 state' ?|= eq d /\ disk1 state' ?|= eq d
+             end;
+     recovered := fun _ state' =>
+                  disk0 state' ?|= eq (diskUpd d a b) /\
+                  disk1 state' ?|= eq (diskUpd d a b) \/
+                  disk0 state' ?|= eq (diskUpd d a b) /\
+                  disk1 state' ?|= eq d \/
+                  disk0 state' ?|= eq d /\ disk1 state' ?|= eq d |})
+    (fixup a) td.recover td.abstr.
+Proof.
+(unfold fixup; intros).
+step.
+(destruct r; try step).
+(destruct r; try step).
+(destruct (b == v); subst; try step).
+step.
+(destruct r; simplify; finish).
+Qed.
+Theorem fixup_wrong_addr_ok :
+  forall a,
+  proc_spec
+    (fun '(d, b, a') state =>
+     {|
+     pre := a < diskSize d /\
+            a' < a /\
+            disk0 state ?|= eq (diskUpd d a' b) /\ disk1 state ?|= eq d;
+     post := fun r state' =>
+             match r with
+             | Continue =>
+                 disk0 state' ?|= eq (diskUpd d a' b) /\
+                 disk1 state' ?|= eq d
+             | RepairDoneOrFailed =>
+                 disk0 state' ?|= eq d /\ disk1 state' ?|= eq d \/
+                 disk0 state' ?|= eq (diskUpd d a' b) /\
+                 disk1 state' ?|= eq (diskUpd d a' b)
+             end;
+     recovered := fun _ state' =>
+                  disk0 state' ?|= eq (diskUpd d a' b) /\
+                  disk1 state' ?|= eq d \/
+                  disk0 state' ?|= eq d /\ disk1 state' ?|= eq d |})
+    (fixup a) td.recover td.abstr.
+Proof.
+(unfold fixup; intros).
+step.
+(destruct r; try step).
+(destruct r; try step).
+(destruct (v == v0); subst).
+-
+step.
+-
+step.
+Unshelve.
+{
+auto.
+}
+exact (fun _ => True).
+Qed.
+Theorem fixup_ok :
+  forall a,
+  proc_spec
+    (fun '(d, s) state =>
+     {|
+     pre := a < diskSize d /\
+            match s with
+            | FullySynced => disk0 state ?|= eq d /\ disk1 state ?|= eq d
+            | OutOfSync a' b =>
+                a' <= a /\
+                disk0 state ?|= eq (diskUpd d a' b) /\ disk1 state ?|= eq d
+            end;
+     post := fun r state' =>
+             match s with
+             | FullySynced => disk0 state' ?|= eq d /\ disk1 state' ?|= eq d
+             | OutOfSync a' b =>
+                 match r with
+                 | Continue =>
+                     a' < a /\
+                     disk0 state' ?|= eq (diskUpd d a' b) /\
+                     disk1 state' ?|= eq d \/
+                     disk0 state' ?|= eq (diskUpd d a' b) /\
+                     disk1 state' ?|= eq (diskUpd d a' b)
+                 | RepairDoneOrFailed =>
+                     disk0 state' ?|= eq d /\ disk1 state' ?|= eq d \/
+                     disk0 state' ?|= eq (diskUpd d a' b) /\
+                     disk1 state' ?|= eq (diskUpd d a' b)
+                 end
+             end;
+     recovered := fun _ state' =>
+                  match s with
+                  | FullySynced =>
+                      disk0 state' ?|= eq d /\ disk1 state' ?|= eq d
+                  | OutOfSync a' b =>
+                      disk0 state' ?|= eq (diskUpd d a' b) /\
+                      disk1 state' ?|= eq (diskUpd d a' b) \/
+                      disk0 state' ?|= eq (diskUpd d a' b) /\
+                      disk1 state' ?|= eq d \/
+                      disk0 state' ?|= eq d /\ disk1 state' ?|= eq d
+                  end |}) (fixup a) td.recover td.abstr.
+Proof.
+(spec_intros; simplify).
+(destruct s; intuition eauto).
+-
+(spec_case fixup_equal_ok; simplify; finish).
+-
+(apply PeanoNat.Nat.lt_eq_cases in H0; intuition).
++
+(spec_case fixup_wrong_addr_ok; simplify; finish).
+(repeat apply exists_tuple2; simpl).
+exists d,b,a0.
+(simplify; finish).
+(destruct v; finish).
++
+(spec_case fixup_correct_addr_ok; simplify; finish).
+exists d,b.
+(simplify; finish).
+(destruct v; finish).
+Restart.
+(intros).
+step_proc.
+(destruct a'; simpl in *).
+(destruct d0; intuition idtac).
+-
+(simplify; finish).
+(destruct r; try step).
+(destruct r; try step).
+(destruct (v == v0); try step).
+-
+(simplify; finish).
+(destruct r; try step).
+(destruct r; try step).
+(destruct (v == v0); try step).
+*
+(assert (a0 < a \/ a0 = a) by lia; intuition auto; simplify).
+*
+intuition eauto.
+{
+step.
 (* Auto-generated comment: Succeeded. *)
 
